All fst dependencies removed

Proofs/Spec.GC_part14.fsti
@@ -706,40 +706,172 @@ let objects2_property_lemma2  (g:heap{(Seq.length (objects2 0UL g) > 0)})
                  (ensures (forall x. Seq.mem x (objects2 h_index g) ==> Usize.v x >= Usize.v h_index)) = ()
 
 
-#reset-options "--z3rlimit 100 --max_fuel 1 --max_ifuel 1 --using_facts_from '* -FStar.Seq'"
-#push-options "--split_queries always"
 
-#restart-solver
-
-#restart-solver
-
-
-val objects2_sweep_lemma3 : (h_index: hp_addr) ->
-                            (g:heap{Seq.length (objects2 0UL g) > 0 /\
+let objects2_sweep_lemma1  (h_index: hp_addr)
+                           (g:heap{Seq.length (objects2 0UL g) > 0 /\
                                    Seq.mem h_index (objects2 0UL g)/\ 
-                                  (Seq.length (objects2 h_index g) > 0)}) ->
-                   Lemma
-                   (ensures 
+                                  (Seq.length (objects2 h_index g) > 0)}) 
+                  :Lemma
+                   (ensures (let wz =  getWosize (read_word g h_index) in
+                             let h_index_new =  Usize.add h_index (Usize.mul (Usize.add wz 1UL) mword) in
+                             let f_index_new =  Usize.add h_index_new mword in
+                             Usize.v f_index_new <> heap_size)) = ()
+
+
+#restart-solver
+
+let wosize_plus_one_times_mword_multiple_of_mword5 (wz:wosize)
+                     :Lemma
+                      (ensures (Usize.v (Usize.mul (Usize.add wz 1UL) mword) % Usize.v mword == 0)) = ()
+
+
+
+
+let objects2_sweep_lemma2  (h_index: hp_addr)
+                           (g:heap{Seq.length (objects2 0UL g) > 0 /\
+                                   Seq.mem h_index (objects2 0UL g)/\
+                                  (Seq.length (objects2 h_index g) > 0)})
+                  :Lemma
+                  (requires (let wz =  getWosize (read_word g h_index) in
+                             let h_index_new =  Usize.add h_index (Usize.mul (Usize.add wz 1UL) mword) in
+                             let f_index_new =  Usize.add h_index_new mword in
+                             Usize.v f_index_new <> heap_size))
+                   (ensures
                    (let wz =  getWosize (read_word g h_index) in
                     let h_index_new =  Usize.add h_index (Usize.mul (Usize.add wz 1UL) mword) in
                     let f_index_new =  Usize.add h_index_new mword in
-                    Usize.v f_index_new >= heap_size ==> ~(Seq.mem h_index_new (objects2 h_index g))))
+                    Usize.v f_index_new >= heap_size ==> ~(Seq.mem h_index_new (objects2 h_index g)))) =
+let wz =  getWosize (read_word g h_index) in
+let h_index_new =  Usize.add h_index (Usize.mul (Usize.add wz 1UL) mword) in
+assert (Seq.mem h_index (objects2 0UL g));
+assert (Seq.length (objects2 0UL g) > 0);
+assert (Seq.length (objects2 0UL g) > 0 ==>
+            (forall x. Seq.mem x (objects2 0UL g) ==> Usize.v (getWosize (read_word g x)) > 0));
+assert  (forall x. Seq.mem x (objects2 0UL g) ==> Usize.v (getWosize (read_word g x)) > 0);
+assert (Usize.v (getWosize (read_word g h_index)) > 0);
 
-val objects2_sweep_lemma4 : (h_index: hp_addr) ->
+assert (Usize.v wz > 0);
+let f_index_new =  Usize.add h_index_new mword in
+ wosize_plus_one_times_mword_multiple_of_mword5 wz;
+ assert (Usize.v (Usize.mul (Usize.add wz 1UL) mword) % Usize.v mword == 0);
+
+ sum_of_multiple_of_mword_is_multiple_of_mword h_index (Usize.mul (Usize.add wz 1UL) mword);
+ sum_of_multiple_of_mword_is_multiple_of_mword h_index_new mword;
+
+ assert (Usize.v (Usize.add h_index_new mword) % Usize.v mword == 0);
+ assert (Usize.v f_index_new % Usize.v mword == 0);
+ if Usize.v h_index_new <= heap_size then //valid heap condition
+  (
+    if Usize.v h_index_new = heap_size then
+    (
+      assert (Seq.length (objects2 h_index g) == 1);
+      assert (Seq.mem h_index (objects2 h_index g));
+      assert (~(Seq.mem h_index_new (objects2 h_index g)));
+      assert (Usize.v f_index_new >= heap_size);
+      ()
+    )
+    else
+    (
+      assert (Usize.v h_index_new < heap_size);
+      assert (Usize.v f_index_new < heap_size \/
+              Usize.v f_index_new == heap_size (*\/
+              Usize.v f_index_new > heap_size*)) ;
+      if Usize.v f_index_new < heap_size then
+      (
+        ()
+      )
+      else
+      (
+        assert (Usize.v f_index_new == heap_size);
+        ()
+      )
+    )
+  )
+ else
+ (
+   assert (Seq.length (objects2 h_index g) > 0);
+   ()
+ )
+
+ let objects2_sweep_lemma3  (h_index: hp_addr)
                            (g:heap{Seq.length (objects2 0UL g) > 0 /\
-                                   Seq.mem h_index (objects2 0UL g)/\ 
-                                  (Seq.length (objects2 h_index g) > 0)}) ->
-                   Lemma
-                   (requires 
+                                   Seq.mem h_index (objects2 0UL g)/\
+                                  (Seq.length (objects2 h_index g) > 0)})
+                  :Lemma
+                   (ensures
+                   (let wz =  getWosize (read_word g h_index) in
+                    let h_index_new =  Usize.add h_index (Usize.mul (Usize.add wz 1UL) mword) in
+                    let f_index_new =  Usize.add h_index_new mword in
+                    Usize.v f_index_new >= heap_size ==> ~(Seq.mem h_index_new (objects2 h_index g)))) =
+objects2_sweep_lemma1 h_index g;
+objects2_sweep_lemma2 h_index g;
+()
+
+let objects2_sweep_lemma4  (h_index: hp_addr)
+                           (g:heap{Seq.length (objects2 0UL g) > 0 /\
+                                   Seq.mem h_index (objects2 0UL g)/\
+                                  (Seq.length (objects2 h_index g) > 0)})
+                  :Lemma
+                   (requires
                      (let wz =  getWosize (read_word g h_index) in
                      let h_index_new =  Usize.add h_index (Usize.mul (Usize.add wz 1UL) mword) in
                      (~(Seq.mem h_index_new (objects2 h_index g)))))
-                   
-                   (ensures 
+
+                   (ensures
                      (let wz =  getWosize (read_word g h_index) in
                      let h_index_new =  Usize.add h_index (Usize.mul (Usize.add wz 1UL) mword) in
                      let f_index_new =  Usize.add h_index_new mword in
-                     Seq.length (objects2 h_index g) == 1))
+                     Seq.length (objects2 h_index g) == 1)) =
+let wz =  getWosize (read_word g h_index) in
+let h_index_new =  Usize.add h_index (Usize.mul (Usize.add wz 1UL) mword) in
+if Usize.v wz = 0 then
+(
+  ()
+)
+else
+(
+  if Usize.v h_index_new <= heap_size then
+  (
+    if Usize.v h_index_new = heap_size then
+    (
+      ()
+    )
+    else
+    (
+      assert (Usize.v h_index_new < heap_size);
+      let f_index_new =  Usize.add h_index_new mword in
+      assert (Usize.v h_index_new < heap_size);
+      wosize_plus_times_mword_multiple_of_mword3 wz;
+      assert (Usize.v (Usize.mul (Usize.add wz 1UL) mword) % Usize.v mword == 0);
+      sum_of_multiple_of_mword_is_multiple_of_mword h_index (Usize.mul (Usize.add wz 1UL) mword);
+      assert ((Usize.v h_index + Usize.v (Usize.mul (Usize.add wz 1UL) mword)) % Usize.v mword == 0);
+      assert (h_index_new ==  Usize.add h_index (Usize.mul (Usize.add wz 1UL) mword));
+      assert (Usize.v h_index_new == Usize.v h_index + Usize.v (Usize.mul (Usize.add wz 1UL) mword));
+      assert (Usize.v h_index_new % Usize.v mword == 0);
+
+      assert ((~(Seq.mem h_index_new (objects2 h_index g))));
+      assert (is_hp_addr h_index_new);
+      let f' =  objects2 h_index_new g in
+      lemma_tl h_index f';
+      let f'' = cons h_index f' in
+      assert (f'' == objects2 h_index g);
+      assert ((~(Seq.mem h_index_new (objects2 h_index g))));
+      assert (forall x. Seq.mem x (objects2 h_index g) ==> Usize.v x >= Usize.v h_index);
+      assert  ((forall x y. Seq.mem x (objects2 h_index g) /\
+                                                   (Usize.v y >= Usize.v x + Usize.v mword) /\
+                                                   (Usize.v y <= Usize.v x + (((Usize.v (getWosize (read_word g x)) + 1) * Usize.v mword) - 1)) ==>
+                                                   ~(Seq.mem y (objects2 h_index g))));
+      assert (Seq.length f' == 0);
+      assert (Seq.length (cons h_index f') == 1);
+      assert (Seq.length f'' == 1);
+      ()
+    )
+  )
+  else
+  (
+    ()
+  )
+)
 
 
 #reset-options "--z3rlimit 100 --max_fuel 1 --max_ifuel 1 --using_facts_from '* -FStar.Seq'"
